code/ecdsap256sha2/Hacl.Impl.P256.LowLevel.fst
@@ -31,11 +31,12 @@ let prime256_buffer: x: ilbuffer uint64 (size 4) {witnessed #uint64 #(size 4) x 
 inline_for_extraction noextract
 val reduction_prime256_2prime256_with_carry_impl: cin: uint64 -> x: felem -> result: felem ->
   Stack unit 
-    (requires fun h -> live h x /\ live h result /\  eq_or_disjoint x result /\ 
+    (requires fun h -> live h x /\ live h result /\ eq_or_disjoint x result /\ 
       (as_nat h x + uint_v cin * pow2 256) < 2 * prime)
     (ensures fun h0 _ h1 -> 
       modifies (loc result) h0 h1 /\ 
-      as_nat h1 result = (as_nat h0 x + uint_v cin * pow2 256) % prime
+      as_nat h1 result < prime /\
+      as_nat_elem h1 result = (as_nat h0 x + uint_v cin * pow2 256) % prime
     )  
 
 
