specs/ecdsap256sha2/Spec.P256.Intermediate.fst
@@ -16,14 +16,6 @@ open Spec.P256.Jacobian
 #set-options "--fuel 0 --ifuel 0 --z3rlimit 100"
 
 noextract
-let basePoint : pointJ =
-  assert_norm (0x6B17D1F2E12C4247F8BCE6E563A440F277037D812DEB33A0F4A13945D898C296 < prime);
-  (0x6B17D1F2E12C4247F8BCE6E563A440F277037D812DEB33A0F4A13945D898C296,
-   0x4FE342E2FE1A7F9B8EE7EB4A7C0F9E162BCE33576B315ECECBB6406837BF51F5,
-   1)
-
-
-noextract
 let _point_double (p:pointJ) : pointJ =
   let x, y, z = p in
   let s = (4 * x * y * y) % prime in
@@ -152,7 +144,7 @@ let scalar_multiplication k p =
 val secret_to_public: scalar -> pointJ
 let secret_to_public k =
   let pai = (0, 0, 0) in
-  let q, f = montgomery_ladder_spec k (pai, basePoint) in
+  let q, f = montgomery_ladder_spec k (pai, toJacobian (base)) in
   _norm q
 
 
